You are given a list of non-negative integers, a1, a2, ..., an, and a target, S. Now you have 2 symbols + and -. For each integer, you should choose one from + and - as its new symbol.

Find out how many ways to assign symbols to make sum of integers equal to target S.

Example 1:
```
Input: nums is [1, 1, 1, 1, 1], S is 3. 
Output: 5
Explanation: 

-1+1+1+1+1 = 3
+1-1+1+1+1 = 3
+1+1-1+1+1 = 3
+1+1+1-1+1 = 3
+1+1+1+1-1 = 3

There are 5 ways to assign symbols to make the sum of nums be target 3.
 ```

Constraints:
```
The length of the given array is positive and will not exceed 20.
The sum of elements in the given array will not exceed 1000.
Your output answer is guaranteed to be fitted in a 32-bit integer.
```
```java
class Solution {
    public int findTargetSumWays(int[] nums, int S) {
        int sum=0;
        for(int i=0;i<nums.length;i++){
            sum+=nums[i];
        }
        int subsetSum=(sum+S)/2;
        if((sum+S)%2!=0 || sum<S) return 0;
        int[][] dp=new int[nums.length+1][subsetSum+1];
        dp[0][0]=1;
        /*
        The below is specially for test cases with 0 as we if we have 0 anywhere in array so that will be added to each subset as adding 0 wont make a difference so lets take test case 0,0,0,0,0,0,1 so 
        if i want to form sum 1 , subsets can be 0+1,0+0+1 so on. SO what we are doing is if we get a 0 we will mutliply the number of subsets we got till ith index with 2 as 0 will be added to all of them . multiplying 2 because either we can include it or exclude it sum is gona remain same.
        */
        for(int i=1;i<=nums.length;i++){
            if(nums[i-1]==0){
                dp[i][0]=2*dp[i-1][0];
            }
            else{
                dp[i][0]=dp[i-1][0];
            }
        }
        for(int i=1;i<dp.length;i++){
            for(int j=1;j<dp[0].length;j++){
                if(j-nums[i-1]>=0){
                    dp[i][j]=dp[i-1][j-nums[i-1]]+dp[i-1][j];
                }
                else{
                    dp[i][j]=dp[i-1][j];
                }
            }
        }
        return dp[dp.length-1][dp[0].length-1];
    }
}
/*
sum-sum1=s
sum-(-sum1)=total
2sum=total+s
sum=(total+s/2)
 
  0 1 2 3 4
0 1 0 0 0 0 
1 1 1 0 0 0  
1 1 2 1 0 0
1 1 3 3 1 0 
1 1 4 6 4 1  
1 1 5 10 10 5 
 
 */   
```
